Adjusted perf axioms; tweaks to single round proof

ironfleet/src/Dafny/Distributed/Common/Framework/Performance.s.dfy
@@ -7,7 +7,7 @@ abstract module Performance_s {
   import opened Collections__Seqs_i
   import opened DS_s : DistributedSystem_s
 
-  datatype PerfExpr = PerfStep(hstep:HostStep)| PerfVoid | PerfZero | PerfAdd(prs:multiset<PerfExpr>) | PerfMax(prs:multiset<PerfExpr>)
+  datatype PerfExpr = PerfDelivery | PerfStep(hstep:HostStep)| PerfVoid | PerfZero | PerfAdd(prs:multiset<PerfExpr>) | PerfMax(prs:multiset<PerfExpr>)
 
   function PerfAdd2(p1:PerfExpr, p2:PerfExpr) : PerfExpr
     ensures p1.PerfAdd? ==> PerfEq(PerfAdd2(p1, p2), PerfAdd(multiset{p2} + p1.prs))
@@ -33,11 +33,20 @@ abstract module Performance_s {
     // ensures forall prs :: p1.PerfAdd? && PerfAdd(prs) in p1.prs && p2 == PerfAdd(p1.prs + prs - multiset{PerfAdd(prs)}) ==> PerfEq(p1, p2)
     // ensures p1.PerfAdd? ==> (forall pr :: pr in p1.prs && pr.PerfAdd? && p2 == PerfAdd(p1.prs + pr.prs - multiset{PerfAdd(pr.prs)}) ==> PerfEq(p1, p2))
 
-  lemma PerfProperties()
+    predicate {:axiom} PerfLe(p1: PerfExpr, p2:PerfExpr)
+
+  lemma {:axiom} PerfProperties()
     // ensures forall p1, p2 :: p1.PerfAdd? ==> 
     ensures forall p1, p2, p1', p2' :: PerfEq(p1, p1') && PerfEq(p2, p2') ==> PerfEq(PerfAdd2(p1, p2), PerfAdd2(p1', p2'));
-    ensures forall p1, p2, p3 :: PerfEq(p1, p2) && PerfEq(p2, p3) ==> PerfEq(p1, p3);
-  {
+    ensures forall p1, p2 :: (forall p1' :: PerfEq(p1, p1') ==> PerfEq(PerfAdd2(p1, p2), PerfAdd2(p1', p2)));
 
-  }
+    ensures forall p1, p2, p3 :: PerfEq(p1, p2) && PerfEq(p2, p3) ==> PerfEq(p1, p3);
+    ensures forall p1, p2 :: PerfEq(p2, PerfVoid) ==> PerfEq(PerfMax(multiset{p1, p2}), PerfMax(multiset{p1}));
+    ensures forall p1, p2, p3 :: PerfEq(PerfAdd2(p1, PerfAdd2(p2, p3)), PerfAdd(multiset{p1, p2, p3}));
+    ensures forall p1, p2, p3 :: PerfEq(p1, p2) ==> (PerfEq(p1, p3) <==> PerfEq(p2, p3));
+
+    ensures forall p1 : PerfExpr, p2 : PerfExpr {:trigger PerfAdd2(p1, p2)} :: (p1.PerfAdd? ==> PerfEq(PerfAdd2(p1, p2), PerfAdd(p1.prs + multiset{p2})));
+
+    ensures forall prs {:trigger PerfMax(prs)} :: PerfEq(PerfMax(prs), PerfMax(prs - multiset{PerfVoid}));
+    ensures forall p1 {:trigger PerfMax(multiset{p1})} :: PerfEq(PerfMax(multiset{p1}), p1)
 }
