ironfleet/src/Dafny/Distributed/Protocol/Lock/PerformanceProof/TaggedGLS.i.dfy
@@ -48,7 +48,19 @@ datatype TaggedGLS_State = TaggedGLS_State(
     reads *
   {
     LS_NextOneServer(UntagLS_State(tls), UntagLS_State(tls'), id, UntagLIoOpSeq(ios), hstep)
-      && (var recvTime := PerfMax(multiset(GetReceivePRs(ios)) + multiset{tls.t_servers[id].pr});
+      && (
+      if |ios| > 0 && ios[0].LIoOpReceive? then
+      (var deliveryTime := PerfAdd2(ios[0].r.msg.pr, PerfDelivery);
+      var handlerStartTime := PerfMax(multiset{deliveryTime, tls.t_servers[id].pr});
+      var totalTime := PerfAdd2(handlerStartTime, PerfStep(GrantStep));
+      totalTime == tls'.t_servers[id].pr)
+      else
+        var totalTime := PerfAdd2(tls.t_servers[id].pr, PerfStep(GrantStep));
+        totalTime == tls'.t_servers[id].pr
+      )
+
+      && (var deliveryTime := PerfMax(multiset(GetReceivePRs(ios)));
+      var recvTime := PerfAdd2(deliveryTime, PerfDelivery);
       var totalTime := PerfAdd2(recvTime, PerfStep(hstep));
       tls'.t_servers[id].pr == totalTime
       )
